Experiments/SR/Checker/SRThm.lean
@@ -15,7 +15,6 @@ namespace Trestle.SR
 
 open RangeArray PPA PS
 open Trestle Trestle.Model PropFun Trestle.Parsing
-open Except
 
 /-
 
@@ -62,34 +61,34 @@ theorem cnfAsListToPropFun_nil : cnfAsListToPropFun [] = ⊤ := by
   simp [cnfAsListToPropFun]
 
 @[simp]
-theorem cnfAsListToPropFun_cons_none (Cs : List (Option (List ILit))) :
-  cnfAsListToPropFun (none :: Cs) = cnfAsListToPropFun Cs := by
+theorem cnfAsListToPropFun_cons_none (Cs : List (Option (List ILit)))
+  : cnfAsListToPropFun (none :: Cs) = cnfAsListToPropFun Cs := by
   simp [cnfAsListToPropFun, all]
 
 @[simp]
-theorem cnfAsListToPropFun_cons_some (C : List ILit) (Cs : List (Option (List ILit))) :
-  cnfAsListToPropFun (some C :: Cs) = clauseAsListToPropFun C ⊓ cnfAsListToPropFun Cs := by
+theorem cnfAsListToPropFun_cons_some (C : List ILit) (Cs : List (Option (List ILit)))
+  : cnfAsListToPropFun (some C :: Cs) = clauseAsListToPropFun C ⊓ cnfAsListToPropFun Cs := by
   simp [cnfAsListToPropFun, all]
 
 @[simp]
-theorem cnfAsListToPropFun_cons (C : Option (List ILit)) (Cs : List (Option (List ILit))) :
-  cnfAsListToPropFun (C :: Cs) =
+theorem cnfAsListToPropFun_cons (C : Option (List ILit)) (Cs : List (Option (List ILit)))
+  : cnfAsListToPropFun (C :: Cs) =
     (match C with
     | none => ⊤
     | some C => clauseAsListToPropFun C) ⊓ cnfAsListToPropFun Cs := by
   cases C <;> simp
 
 @[simp]
-theorem cnfAsListToPropFun_append (Cs₁ Cs₂ : List (Option (List ILit))) :
-  cnfAsListToPropFun (Cs₁ ++ Cs₂) = cnfAsListToPropFun Cs₁ ⊓ cnfAsListToPropFun Cs₂ := by
+theorem cnfAsListToPropFun_append (Cs₁ Cs₂ : List (Option (List ILit)))
+  : cnfAsListToPropFun (Cs₁ ++ Cs₂) = cnfAsListToPropFun Cs₁ ⊓ cnfAsListToPropFun Cs₂ := by
   induction Cs₁ with
   | nil => simp
   | cons C Cs₁ ih =>
     cases C <;> simp [ih, inf_assoc]
 
 @[simp]
-theorem cnfAsListToPropFun_replicate_none (n : Nat) :
-    cnfAsListToPropFun (List.replicate n none) = ⊤ := by
+theorem cnfAsListToPropFun_replicate_none (n : Nat)
+  : cnfAsListToPropFun (List.replicate n none) = ⊤ := by
   induction n with
   | zero => simp
   | succ n ih =>
@@ -97,15 +96,15 @@ theorem cnfAsListToPropFun_replicate_none (n : Nat) :
     exact ih
 
 theorem clausePropFun_ge_of_mem {C : List ILit} {l : ILit}
-    : l ∈ C → l.toPropFun ≤ clauseAsListToPropFun C := by
+  : l ∈ C → l.toPropFun ≤ clauseAsListToPropFun C := by
   intro h
   rw [clauseAsListToPropFun_eq_toPropFun]
   apply Clause.toPropFun_mem_le
   simp only [List.mem_toArray, h]
 
 theorem cnfPropFun_le_of_mem {Cs : List (Option (List ILit))} {C : List ILit} {i : Nat}
-      {hi : i < Cs.length} :
-    Cs.get ⟨i, hi⟩ = some C → cnfAsListToPropFun Cs ≤ clauseAsListToPropFun C := by
+      {hi : i < Cs.length}
+    : Cs.get ⟨i, hi⟩ = some C → cnfAsListToPropFun Cs ≤ clauseAsListToPropFun C := by
   intro h
   simp [cnfAsListToPropFun_eq_toPropFun]
   induction Cs generalizing i with
@@ -128,6 +127,43 @@ theorem cnfPropFun_le_of_mem {Cs : List (Option (List ILit))} {C : List ILit} {i
         have := ih h
         apply le_trans _ this
         simp
+
+theorem cnfPropFun_drop_le_of_le (Cs : List (Option (List ILit))) {n₁ n₂ : Nat}
+  : n₁ ≤ n₂ → cnfAsListToPropFun (List.drop n₁ Cs) ≤ cnfAsListToPropFun (List.drop n₂ Cs) := by
+  intro hn
+  induction Cs generalizing n₁ n₂ with
+  | nil => simp
+  | cons C Cs ih =>
+    cases n₁ with
+    | zero =>
+      cases n₂ with
+      | zero => simp
+      | succ n₂ =>
+        replace ih := ih (Nat.zero_le n₂)
+        simp at ih
+        simp
+        exact inf_le_of_right_le ih
+    | succ n₁ =>
+      cases n₂ with
+      | zero => contradiction
+      | succ n₂ =>
+        replace ih := ih (Nat.le_of_succ_le_succ hn)
+        simp [ih]
+
+theorem cnfPropFun_drop_succ_of_none {Cs : List (Option (List ILit))} {n : Nat} (hn : n < Cs.length)
+  : Cs[n] = none → cnfAsListToPropFun (List.drop (n + 1) Cs) = cnfAsListToPropFun (List.drop n Cs) := by
+  intro h
+  induction Cs generalizing n with
+  | nil => simp at hn
+  | cons C Cs ih =>
+    cases n with
+    | zero =>
+      simp at h; subst h
+      simp
+    | succ n =>
+      simp at h hn
+      replace ih := ih hn h
+      simp [ih]
 
 theorem cnfPropFun_le_set_none {Cs : List (Option (List ILit))}
   {i : Nat} (hi : i < Cs.length) :
@@ -211,39 +247,99 @@ theorem assumeNegatedCandidateFor_eq_assumeNegatedClauseFor {F : RangeArray ILit
   simp [assumeNegatedCandidateFor, assumeNegatedClauseFor]
   exact @assumeNegatedCandidateFor.loop.aux _ _ _ _ h_models bumps 0 F.usize h_models.h_size₂
 
+/-! # iget -/
+
+def iget {F : RangeArray ILit} {Ls} {L : List ILit} (h_models : models F Ls L) (i : Nat) (C : List ILit) : Prop :=
+  if hi : i < F.size then Ls.get ⟨i, h_models.h_size₁ ▸ hi⟩ = some C else C = L
+
+theorem iget_lt {F : RangeArray ILit} {Ls} {L : List ILit} {h_models : models F Ls L}
+    {i : Nat} {C : List ILit} (h_iget : iget h_models i C) (hi : i < F.size)
+  : Ls.get ⟨i, h_models.h_size₁ ▸ Nat.lt_of_not_ge (not_le.mpr hi)⟩ = some C := by
+  simp [iget, hi] at h_iget
+  exact h_iget
+
+theorem iget_eq {F : RangeArray ILit} {Ls} {L : List ILit} {h_models : models F Ls L} {C : List ILit}
+  : iget h_models F.size C → C = L := by
+  simp [iget]
+
+@[simp]
+theorem iget_Fsize {F : RangeArray ILit} {Ls} {L : List ILit} (h_models : models F Ls L)
+    : iget h_models F.size L := by
+  simp [iget]
+
+theorem iget_of_eq_some {F : RangeArray ILit} {Ls} {L C} (h_models : models F Ls L) {i} {hi : i < Ls.length}
+    : Ls[i] = some C → iget h_models i C := by
+  simp [iget, h_models.h_size₁ ▸ hi]
+
 theorem assumeRATClause.loop.aux {F : RangeArray ILit} {τ : PPA} {σ : PS}
-    {Ls : List (Option (List ILit))} {L : List ILit} (h_models : models F Ls L)     -- models
-    {i : Nat} (hi : i < F.size)                                                     -- Clause index
-    {C : List ILit} (hC : Ls.get ⟨i, h_models.h_size₁ ▸ hi⟩ = some C)               -- Clause at i
+    {Ls : List (Option (List ILit))} {L : List ILit} (h_models : models F Ls L)
+    {i : Nat} (hi : i ≤ F.size)
+    {C : List ILit} (hC : iget h_models i C)
     {j k : Nat}
   : k = C.length - j →
-    match assumeRATClause.loop F i σ ((F.index i hi) + j) τ with
+    match assumeRATClause.loop F i hi σ ((F.index! i) + j) τ with
     -- If we exit early, then τ satisfies the clause under the substitution, and τ is unchanged
     | .error τ' => τ.toPropFun ≤ PropFun.substL (clauseAsListToPropFun ((C.drop j))) σ.toSubst ∧ extendsFor τ τ' 0
     -- If we make it to the end, then τ' has been assumed by the negated candidate under the substitution
     | .ok τ' => τ'.toPropFun = ↑τ ⊓ (PropFun.substL (clauseAsListToPropFun ((C.drop j))) σ.toSubst)ᶜ ∧ extendsFor τ τ' 0 := by
   intro hk
   have hiL := h_models.h_size₁ ▸ hi
-  have hi' := h_models.h_sizes (hiL) hC
   induction k generalizing τ j with
   | zero =>
     have h_le₁ := Nat.le_of_sub_eq_zero hk.symm
     unfold assumeRATClause.loop
-    have hj := hi' ▸ h_le₁
-    simp [rsize] at hj
-    rw [add_comm j] at hj
-    simp [not_lt_of_ge hj, List.drop_eq_nil_iff.mpr h_le₁]
+    simp [List.drop_eq_nil_iff.mpr h_le₁]
+    by_cases hi' : i = F.size
+    · subst hi'
+      have := iget_eq hC; subst this
+      have := h_models.h_size₂
+      rw [usize] at this
+      have : F.dsize + j ≥ F.data.size := by omega
+      simp [not_lt_of_ge this]
+    · replace hi' := Nat.lt_of_le_of_ne hi hi'
+      replace hC := iget_lt hC hi'
+      have hiF := h_models.h_sizes (h_models.h_size₁ ▸ hi') hC
+      have hj := hiF ▸ h_le₁
+      simp [rsize] at hj
+      rw [add_comm j] at hj
+      simp [Nat.ne_of_lt hi']
+      have : F.index! (i + 1) ≤ F.index! i + j := by
+        conv => rhs; rw [index!]
+        simp [hi']
+        exact hj
+      simp [not_lt_of_ge this]
   | succ k ih =>
     unfold assumeRATClause.loop
     have hj_lt : j < C.length := by omega
     replace hk : k = C.length - (j + 1) := by omega
-    have : F.index i hi + j < F.index! (i + 1) := by
-      simp [rsize] at hi'
-      omega
-    have hF := h_models.h_agree hiL hC hj_lt
-    rw [oget] at hF
-    simp [this, hF]
-    clear hF
+    -- Do some non-finishing-tactic casework
+    -- Adjust hypotheses based on whether we are processing the candidate or a formula clause
+    by_cases hi' : i = F.size
+    focus
+      subst hi'
+      have this := iget_eq hC; subst this; clear hC
+      have hC := h_models.h_size₂
+      simp [usize] at hC
+      have hj : F.dsize + j < F.data.size := by omega
+      have hFC := h_models.h_uncommitted hj_lt
+      simp [uget] at hFC
+      simp [hj, hFC]
+      clear hFC hj hiL
+    swap
+    focus
+      replace hi := Nat.lt_of_le_of_ne hi hi'
+      replace hiL := h_models.h_size₁ ▸ hi
+      replace hC := iget_lt hC hi
+      have : F.index! i + j < F.index! (i + 1) := by
+        have := h_models.h_sizes hiL hC
+        simp [rsize] at this
+        rw [index_eq_index!] at this
+        omega
+      have hF := h_models.h_agree hiL hC hj_lt
+      simp_rw [oget, index_eq_index!] at hF
+      simp [hi', this, hF]
+      clear hF hiL this
+    all_goals (
     match hσ : σ.litValue C[j] with
     | .inr true =>
       simp
@@ -314,11 +410,12 @@ theorem assumeRATClause.loop.aux {F : RangeArray ILit} {τ : PPA} {σ : PS}
           rw [← List.getElem_cons_drop hj_lt, Clause.toPropFun_cons]
           simp [← litValue_eq, hσ, PSV.toPropFun]
           exact le_sup_of_le_left this
+    )
 
 theorem assumeRATClause_spec {F : RangeArray ILit} (τ : PPA) (σ : PS)
-    {Ls : List (Option (List ILit))} {L : List ILit} (h_models : models F Ls L)     -- models
-    {i : Nat} (hi : i < F.size)                                                     -- Clause index
-    {C : List ILit} (hC : Ls.get ⟨i, h_models.h_size₁ ▸ hi⟩ = some C)               -- Clause at c_idx
+    {Ls : List (Option (List ILit))} {L : List ILit} (h_models : models F Ls L)
+    {i : Nat} (hi : i ≤ F.size)
+    {C : List ILit} (hC : iget h_models i C)
   : match assumeRATClause F i hi σ τ with
     | .error τ' => τ.toPropFun ≤ PropFun.substL (clauseAsListToPropFun C) σ.toSubst ∧ extendsFor τ τ' 0
     | .ok τ' => τ'.toPropFun = ↑τ ⊓ (PropFun.substL (clauseAsListToPropFun C) σ.toSubst)ᶜ ∧ extendsFor τ τ' 0 := by
@@ -326,9 +423,9 @@ theorem assumeRATClause_spec {F : RangeArray ILit} (τ : PPA) (σ : PS)
   exact @assumeRATClause.loop.aux _ _ _ _ _ h_models i hi C hC 0 (C.length) rfl
 
 theorem assumeRATClause_error {F : RangeArray ILit} {τ τ' : PPA} {σ : PS}
-    {Ls : List (Option (List ILit))} {L : List ILit} (h_models : models F Ls L)     -- models
-    {i : Nat} {hi : i < F.size}                                                     -- Clause index
-    {C : List ILit} (hC : Ls.get ⟨i, h_models.h_size₁ ▸ hi⟩ = some C)               -- Clause at c_idx
+    {Ls : List (Option (List ILit))} {L : List ILit} (h_models : models F Ls L)
+    {i : Nat} {hi : i ≤ F.size}
+    {C : List ILit} (hC : iget h_models i C)
   : assumeRATClause F i hi σ τ = .error τ' →
     τ.toPropFun ≤ PropFun.substL (clauseAsListToPropFun C) σ.toSubst ∧ extendsFor τ τ' 0 := by
   intro h
@@ -337,9 +434,9 @@ theorem assumeRATClause_error {F : RangeArray ILit} {τ τ' : PPA} {σ : PS}
   exact this
 
 theorem assumeRATClause_ok {F : RangeArray ILit} {τ τ' : PPA} {σ : PS}
-    {Ls : List (Option (List ILit))} {L : List ILit} (h_models : models F Ls L)     -- models
-    {i : Nat} {hi : i < F.size}                                                     -- Clause index
-    {C : List ILit} (hC : Ls.get ⟨i, h_models.h_size₁ ▸ hi⟩ = some C)               -- Clause at c_idx
+    {Ls : List (Option (List ILit))} {L : List ILit} (h_models : models F Ls L)
+    {i : Nat} {hi : i ≤ F.size}
+    {C : List ILit} (hC : iget h_models i C)
   : assumeRATClause F i hi σ τ = .ok τ' →
     τ'.toPropFun = ↑τ ⊓ (PropFun.substL (clauseAsListToPropFun C) σ.toSubst)ᶜ ∧ extendsFor τ τ' 0 := by
   intro h
@@ -461,11 +558,6 @@ theorem applyUPHint_spec {F : RangeArray ILit} {τ : PPA}
   · have h_hint' := h_models.h_size₁ ▸ h_hint
     simp [h_hint']
 
-@[simp]
-theorem applyUPHints.nil (F : RangeArray ILit) (τ : PPA) (bumps : Nat)
-  : applyUPHints F bumps τ { toList := [] } = ⟨τ, .unit⟩ := by
-  simp [applyUPHints, applyUPHints.loop]
-
 theorem applyUPHints.loop.cons_succ' (F : RangeArray ILit) (τ : PPA) (bumps hint : Nat)
     {hints : List Nat} {i j : Nat}
   : j = hints.length - i →
@@ -579,13 +671,12 @@ theorem applyUPHints_contra {F : RangeArray ILit} {τ τ' : PPA}
 
 /-! # reduce -/
 
-theorem reduce_loop_eq_reduce_loop (F : RangeArray ILit) (σ : PS) (hint : Nat)
-  (h_hint : hint < F.size)
+theorem reduce_loop_eq_reduce_loop (F : RangeArray ILit) (σ : PS) (hint : Nat) (h_hint : hint ≤ F.size)
   {Ls : List (Option (List ILit))} {L : List ILit} (h_models : models F Ls L)
-  {C : List ILit} (hC : Ls.get ⟨hint, h_models.h_size₁ ▸ h_hint⟩ = some C)
-  (b : Bool) {i j : Nat}
-    : j = F.rsize hint h_hint - i →
-        RangeArray.reduce.loop F hint σ.gens σ.mappings σ.generation σ.sizes_eq (F.index hint h_hint + i) b =
+  {C : List ILit} (hC : iget h_models hint C)
+  {i j : Nat} (b : Bool)
+    : j = (if h_hint' : hint = F.size then F.usize else F.rsize hint (Nat.lt_of_le_of_ne h_hint h_hint')) - i →
+        RangeArray.reduce.loop F hint h_hint σ.gens σ.mappings σ.generation σ.sizes_eq (F.index! hint + i) b =
         PS.reduce.loop σ ({ toList := C } : IClause) i b := by
   intro hj
   induction j generalizing i b with
@@ -593,26 +684,56 @@ theorem reduce_loop_eq_reduce_loop (F : RangeArray ILit) (σ : PS) (hint : Nat)
     have h_le := Nat.le_of_sub_eq_zero hj.symm
     unfold RangeArray.reduce.loop
     unfold PS.reduce.loop
-    have h_rsize := h_le
-    have h_rsize' := h_models.h_sizes (h_models.h_size₁ ▸ h_hint) hC
-    simp [rsize, Nat.add_comm i] at h_rsize
-    simp [not_lt_of_ge h_rsize, ← h_rsize']
-    intro h_con
-    omega
+    by_cases h_hint' : hint = F.size
+    · subst h_hint'
+      simp at hj h_le
+      have := iget_eq hC; subst this; clear hC
+      have : F.dsize + i ≥ F.data.size := by omega
+      simp [not_lt_of_ge this]
+      clear this
+      have := h_models.h_size₂
+      intro h_con
+      omega
+    · have h_hint_lt := Nat.lt_of_le_of_ne h_hint h_hint'
+      replace hC := iget_lt hC h_hint_lt
+      have h_rsize := h_models.h_sizes (h_models.h_size₁ ▸ h_hint_lt) hC
+      simp [rsize, h_hint', index_eq_index!] at h_le hj h_rsize
+      have : F.index! hint + i ≥ F.index! (hint + 1) := by omega
+      simp [h_hint', not_lt_of_ge this]
+      intro h_con
+      omega
   | succ j ih =>
-    have hi : i < F.rsize hint h_hint := by omega
-    have hi' := hi
-    have hj' : j = F.rsize hint h_hint - (i + 1) := by omega
-    simp [rsize] at hi'
-    have : F.index hint h_hint + i < F.index! (hint + 1) := by omega
-    have h_rsize' := h_models.h_sizes (h_models.h_size₁ ▸ h_hint) hC
-    have hiC := h_rsize' ▸ hi
     unfold RangeArray.reduce.loop PS.reduce.loop
-    simp [← h_rsize', hi, this]
-    have h_hint' := h_models.h_size₁ ▸ h_hint
-    have h_Fget := h_models.h_agree h_hint' hC hiC
-    simp [oget] at h_Fget
-    simp [h_Fget, seval]
+    simp [seval]
+    rw [Nat.add_assoc]
+    replace ih := fun b => ih (i := i + 1) b (by omega)
+    by_cases hi' : hint = F.size
+    focus
+      -- Do some non-finishing-tactic casework
+      -- Adjust hypotheses based on whether we are processing the candidate or a formula clause
+      subst hi'
+      have := iget_eq hC; subst this; clear hC
+      simp [usize] at hj
+      have hC_len := h_models.h_size₂
+      simp [usize] at hC_len
+      have hFC := h_models.h_uncommitted (i := i) (by omega)
+      simp [uget] at hFC
+      have hiC : i < C.length := by omega
+      have : F.dsize + i < F.data.size := by omega
+      simp [hFC, hiC, this]
+      simp only [index!, lt_self_iff_false, ↓reduceDIte] at ih
+    swap
+    focus
+      have h_hint' := Nat.lt_of_le_of_ne h_hint hi'
+      replace hC := iget_lt hC h_hint'
+      have hC_len := h_models.h_sizes (h_models.h_size₁ ▸ h_hint') hC
+      simp [hi', rsize, index_eq_index!] at hj hC_len
+      have hiC : i < C.length := by omega
+      have hFC := h_models.h_agree (h_models.h_size₁ ▸ h_hint') hC hiC
+      simp [oget, index_eq_index!] at hFC
+      have : F.index! hint + i < F.index! (hint + 1) := by omega
+      simp [hi', hiC, hFC, this]
+    all_goals (
     match hσ : σ.litValue C[i] with
     | .inr true =>
       -- Satisfied case
@@ -632,8 +753,7 @@ theorem reduce_loop_eq_reduce_loop (F : RangeArray ILit) (σ : PS) (hint : Nat)
       simp [h_size, h_gen, h_map]
       by_cases h_pol : LitVar.polarity C[i]
       <;> simp [h_pol, MAPPED_TRUE, MAPPED_FALSE]
-      <;> have := ih true hj'
-      <;> rwa [← Nat.add_assoc] at this
+      <;> exact ih true
     | .inl lit =>
       by_cases h_lit : C[i] = lit
       -- Id-mapped case
@@ -654,16 +774,13 @@ theorem reduce_loop_eq_reduce_loop (F : RangeArray ILit) (σ : PS) (hint : Nat)
                 simp at h_map
                 have : (n / 2 + 1) * 2 = n + 1 + 1 := by omega
                 simp [h_map, IVarToMappedNat, this]
-                rw [Nat.add_assoc]
-                exact ih b hj'
+                exact ih b
               · simp at hσ
                 subst hσ
                 simp at h_pol
-            · simp [h_gen] at hσ ⊢
-              rw [Nat.add_assoc]
-              exact ih b hj'
-          · rw [Nat.add_assoc]
-            exact ih b hj'
+            · simp [h_gen]
+              exact ih b
+          · exact ih b
         · by_cases h_lt : lit.index < σ.gens.size
           <;> simp [h_lt] at hσ ⊢
           · by_cases h_gen : σ.generation ≤ σ.gens[lit.index]
@@ -678,15 +795,12 @@ theorem reduce_loop_eq_reduce_loop (F : RangeArray ILit) (σ : PS) (hint : Nat)
                 subst hσ
                 have : (n' / 2 + 1) * 2 = n' + 1 + 1 := by omega
                 simp [IVarToMappedNat, this]
-                rw [Nat.add_assoc]
-                exact ih b hj'
+                exact ih b
               · simp at hσ
                 subst hσ
                 simp at h_pol
-            · rw [Nat.add_assoc]
-              exact ih b hj'
-          · rw [Nat.add_assoc]
-            exact ih b hj'
+            · exact ih b
+          · exact ih b
       · have h_size := lt_size_of_litValue_ne_id (σ := σ) (l := C[i]) (by simp [hσ]; exact Ne.symm h_lit)
         have h_gen := ge_gen_of_litValue_ne_id (σ := σ) (l := C[i]) (by simp [hσ]; exact Ne.symm h_lit)
         have h_map := mappings_eq_of_litValue_lit h_lit hσ
@@ -707,16 +821,14 @@ theorem reduce_loop_eq_reduce_loop (F : RangeArray ILit) (σ : PS) (hint : Nat)
             · have : (LitVar.toVar C[i]).val = n / 2 + 1 := by omega
               apply absurd _ h_lit
               simp [← this]
-            · rw [Nat.add_assoc]
-              exact ih true hj'
+            · exact ih true
           · rename_i h_mod
             subst hσ
             clear h_lit
             simp [IVarToMappedNat]
             split <;> rename_i h
             · omega
-            · rw [Nat.add_assoc]
-              exact ih true hj'
+            · exact ih true
         · rw [hC] at hσ
           simp [PSV.fromMappedNat, negateMappedNat] at hσ
           split at hσ
@@ -734,8 +846,7 @@ theorem reduce_loop_eq_reduce_loop (F : RangeArray ILit) (σ : PS) (hint : Nat)
               apply absurd _ h_lit
               rw [hC]
               simp [← this]
-            · rw [Nat.add_assoc]
-              exact ih true hj'
+            · exact ih true
           · rename_i h_mod
             simp at hn'; subst hn'
             simp at h_mod
@@ -745,160 +856,186 @@ theorem reduce_loop_eq_reduce_loop (F : RangeArray ILit) (σ : PS) (hint : Nat)
             simp [IVarToMappedNat]
             split <;> rename_i h
             · omega
-            · rw [Nat.add_assoc]
-              exact ih true hj'
+            · exact ih true
+    ) /- end all_goals -/
 
-theorem reduce_eq_reduce (F : RangeArray ILit) (σ : PS) (hint : Nat)
-  (h_hint : hint < F.size)
+theorem reduce_eq_reduce (F : RangeArray ILit) (σ : PS) (hint : Nat) (h_hint : hint ≤ F.size)
   {Ls : List (Option (List ILit))} {L : List ILit} (h_models : models F Ls L)
-  {C : List ILit} (hC : Ls.get ⟨hint, h_models.h_size₁ ▸ h_hint⟩ = some C)
-    : RangeArray.reduce σ F hint h_hint = PS.reduce σ ({ toList := C } : IClause) := by
+  {C : List ILit} (hC : iget h_models hint C)
+    : RangeArray.reduce F hint h_hint σ = PS.reduce σ ({ toList := C } : IClause) := by
   unfold RangeArray.reduce PS.reduce
-  have := @reduce_loop_eq_reduce_loop F σ hint h_hint _ _ h_models C hC false 0 (F.rsize hint h_hint) rfl
+  have := @reduce_loop_eq_reduce_loop F σ hint h_hint _ _ h_models C hC 0
+    (if h_hint' : hint = F.size then F.usize else F.rsize hint (Nat.lt_of_le_of_ne h_hint h_hint')) false rfl
   simp at this
   exact this
 
-theorem checkLine.loop_ok_aux {line : SRAdditionLine} {F : RangeArray ILit}
+theorem checkLine.loop_true_aux {line : SRAdditionLine} {F : RangeArray ILit}
     {Ls : List (Option (List ILit))} {L : List ILit} (h_models : models F Ls L)
-    {τ τ' : PPA} {σ : PS} {i j cri bc : Nat} :
+    {τ τ' : PPA} --(hτ : τ.toPropFun = (clauseAsListToPropFun L)ᶜ)
+    {σ : PS} {i j cri bc : Nat} (hi : i ≤ F.size) :
   j = F.size - i →
   uniform τ (line.ratHints.size + 1 - bc) →
-    checkLine.loop F line.witnessMaps line.ratHintIndexes line.ratHints line.ratSizesEq σ i cri bc τ = ⟨τ', true⟩ →
+    checkLine.loop F line.witnessMaps line.ratHintIndexes line.ratHints line.ratSizesEq σ i hi cri bc τ = ⟨τ', true⟩ →
     ---- can probably be done in a suffices -----
       (∃ (b : Nat), b ≤ line.ratHints.size + 1 - bc ∧ uniform τ' b)
       ∧ τ'.toPropFun = τ.toPropFun
     ---- suffices -----
-      ∧ ∀ {k : Nat} {hk : k < Ls.length} {C : List ILit},
-        Ls.get ⟨k, hk⟩ = some C → i ≤ k →
-          (cnfAsListToPropFun Ls) ⊓ τ ≤ PropFun.substL (clauseAsListToPropFun C) σ.toSubst := by
+      ∧ (cnfAsListToPropFun Ls) ⊓ τ ≤ PropFun.substL (cnfAsListToPropFun (Ls.drop i)) σ.toSubst
+      ∧ (cnfAsListToPropFun Ls) ⊓ τ ≤ PropFun.substL (clauseAsListToPropFun L) σ.toSubst := by
   intro hj h_uniform
-  simp
   induction j generalizing τ i cri bc with
   | zero =>
-    have hi : i ≥ F.size := Nat.le_of_sub_eq_zero hj.symm
+    -- i = F.size, so we are checking the candidate clause
+    have hi : i = F.size := by omega
+    subst hi
+    clear hj
     unfold loop
-    simp [not_lt.mpr hi]
-    rintro rfl
-    simp
-    use ⟨line.ratHints.size + 1 - bc, le_refl _, h_uniform⟩
-    intro k hk₂ _ _ hk₁
-    rw [← h_models.h_size₁] at hk₂
-    have := lt_of_le_of_lt hk₁ hk₂
-    exact absurd this (not_lt.mpr hi)
+    simp [reduce_eq_reduce F σ F.size (Nat.le_refl _) h_models (iget_Fsize h_models)]
+    match h_reduce : σ.reduce { toList := L } with
+    | .notReduced => simp
+    | .satisfied =>
+      simp
+      rintro rfl
+      simp [reduce_satisfied h_reduce, h_models.h_size₁]
+      exact ⟨_, le_refl _, h_uniform⟩
+    | .reduced =>
+      -- Casework on a successful RAT hint find and assumption
+      simp
+      split <;> rename_i h_bc
+      <;> try simp
+      have hbc : line.ratHints.size + 1 - bc = line.ratHints.size - (bc + 1) + 2 := by omega
+      have h_uniform' := hbc ▸ h_uniform
+      split
+      <;> try simp
+      rename_i ri h_rat h_find_rat_hint
+      split <;> rename_i τ₃ h_assume_rat
+      <;> try simp
+      · rintro rfl
+        rcases assumeRATClause_error h_models (iget_Fsize h_models) h_assume_rat with ⟨hτ_le, hτ_ext⟩
+        rcases uniform_bump_of_uniform_of_extendsFor' h_uniform' hτ_ext with ⟨h_uniform', hτ₃⟩
+        simp [← hτ₃, h_models.h_size₁]
+        use ⟨_, by omega, h_uniform'⟩
+        simp at hτ_le
+        apply le_trans _ hτ_le
+        exact inf_le_right
+      · split <;> rename_i τ₄ h_up
+        <;> try simp
+        rintro rfl
+        rcases assumeRATClause_ok h_models (iget_Fsize h_models) h_assume_rat with ⟨hτ_le, hτ_ext⟩
+        rcases applyUPHints_contra h_models h_up with ⟨h_up_le, h_up_ext⟩
+        replace h_up_ext := extendsFor_trans hτ_ext h_up_ext
+        rcases uniform_bump_of_uniform_of_extendsFor' h_uniform' h_up_ext with ⟨h_uniform', hτ₄⟩
+        simp [← hτ₄, h_models.h_size₁]
+        use ⟨_, by omega, h_uniform'⟩
+        simp at hτ_le h_up_le
+        simp [hτ_le, ← inf_assoc] at h_up_le
+        exact le_iff_inf_compl_eq_bot.mpr h_up_le
   | succ j ih =>
-    unfold loop
-    have hi : i < F.size := by omega
+    have hi_lt : i < F.size := by omega
+    have hi_lt' := h_models.h_size₁ ▸ hi_lt
     have hj' : j = F.size - (i + 1) := by omega
-    simp [hi]
+    unfold loop
+    simp [hi_lt]
     -- Split on whether the ith clause is deleted
     split <;> rename_i h_del
     · -- It's deleted, so no change in the reduction at hint `i`
       intro h_loop
-      rcases ih hj' h_uniform h_loop with ⟨hτ, hpf, hkC⟩
-      use hτ, hpf
-      intro k hk₂ C hC hk₁
-      by_cases hik : i = k
-      · -- if i = k, then the loop body checks the kth clause
-        subst hik
-        clear hk₁
-        rw [(h_models.h_some (h_models.h_size₁ ▸ hi)).mpr ⟨C, hC⟩] at h_del
-        contradiction
-      · -- if i ≠ k, then we use `hkC` from the IH on an earlier reduction
-        exact hkC hC (by omega)
+      rcases ih (Nat.succ_le_of_lt hi_lt) hj' h_uniform h_loop with ⟨hτ, hpf, hL, hC⟩
+      refine ⟨hτ, hpf, ?_, hC⟩
+      clear hτ hpf hC
+      apply le_trans hL
+      apply substL_le_of_le
+      have := eq_none_of_models_of_deleted h_models hi_lt' h_del
+      rw [cnfPropFun_drop_succ_of_none hi_lt' this]
     · -- Not deleted, so we split on the returned result from `reduce`
       simp at h_del
+      rcases (h_models.h_some hi_lt').mp h_del with ⟨C, hC⟩
+      have h_iget := iget_of_eq_some h_models hC
+      simp [reduce_eq_reduce F σ i hi h_models h_iget]
       intro h_loop
-      rcases (h_models.h_some (h_models.h_size₁ ▸ hi)).mp h_del with ⟨C, hC⟩
       split at h_loop <;> rename_i h_reduce
       -- reduce: Satisfied
-      · rcases ih hj' h_uniform h_loop with ⟨hτ, hpf, hkC⟩
-        use hτ, hpf
-        intro k hk C' hC' hik
-        rcases lt_or_eq_of_le hik with (hk₁ | rfl)
-        · exact hkC hC' (by omega)
-        · rw [reduce_eq_reduce F σ i hi h_models hC] at h_reduce
-          have h_reduce := PS.reduce_satisfied h_reduce
-          simp [hC'] at hC
-          subst hC
-          simp [h_reduce]
+      · rcases ih (Nat.succ_le_of_lt hi_lt) hj' h_uniform h_loop with ⟨hτ, hpf, hL, hC⟩
+        refine ⟨hτ, hpf, ?_, hC⟩
+        clear hτ hpf hC
+        replace h_reduce := reduce_satisfied h_reduce
+        simp [← List.getElem_cons_drop hi_lt', hC, h_reduce, hL]
       -- reduce: not reduced
-      · rcases ih hj' h_uniform h_loop with ⟨hτ, hpf, hkC⟩
-        use hτ, hpf
-        intro k hk C hC hik
-        rcases lt_or_eq_of_le hik with (hk₁ | rfl)
-        · exact hkC hC (by omega)
-        · rw [reduce_eq_reduce F σ i hi h_models hC] at h_reduce
-          rw [PS.reduce_notReduced h_reduce]
-          exact inf_le_of_left_le (cnfPropFun_le_of_mem hC)
+      · rcases ih (Nat.succ_le_of_lt hi_lt) hj' h_uniform h_loop with ⟨hτ, hpf, hL, hC⟩
+        refine ⟨hτ, hpf, ?_, hC⟩
+        clear ih hτ hpf hC
+        replace h_reduce := reduce_notReduced h_reduce
+        simp [← List.getElem_cons_drop hi_lt', hC, h_reduce, hL]
+        apply le_trans _ (cnfPropFun_le_of_mem hC)
+        exact inf_le_left
       -- reduce. We continue with the loop by running UP on the reduced clause
       · split at h_loop <;> rename_i h_bc
-        · -- Do we successfully find a RAT hint?
+        <;> try simp at h_loop
+        -- Do we successfully find a RAT hint?
+        split at h_loop
+        <;> try simp at h_loop
+        rename_i ri h_ri h_find_hint
+        -- What's the result of assuming the negation of the reduced clause?
+        split at h_loop
+        <;> rename_i τ'' h_assume
+        · -- Error: the clause is satisfied by σ or τ
+          have h_iget := iget_of_eq_some h_models hC
+          rcases assumeRATClause_error h_models h_iget h_assume with ⟨hτ_le, hτ_ext⟩
+          clear h_assume
+          have : line.ratHints.size + 1 - bc = line.ratHints.size - (bc + 1) + 2 := by omega
+          rcases uniform_bump_of_uniform_of_extendsFor' (this ▸ h_uniform) hτ_ext with ⟨h_uniform'', hτ''⟩
+          clear this
+          have : (line.ratHints.size - (bc + 1) + 1) = line.ratHints.size + 1 - (bc + 1) := by omega
+          rw [this] at h_uniform''
+          clear this
+          rcases ih (Nat.succ_le_of_lt hi_lt) hj' h_uniform'' h_loop with ⟨⟨b, hb₁, hb₂⟩, hpf, hL, hC⟩
+          rw [hτ''] at hτ_le ⊢
+          refine ⟨⟨b, by omega, hb₂⟩, hpf, ?_, hC⟩
+          clear ih h_find_hint h_loop b hb₁ hb₂ hpf hC
+          simp [← List.getElem_cons_drop hi_lt', hC, hL]
+          exact inf_le_of_right_le hτ_le
+        · -- Ok: We have now assumed the negation of the clause under σ
+          rcases assumeRATClause_ok h_models (iget_of_eq_some h_models hC) h_assume with ⟨hτ'', h_ext⟩
+          clear h_assume
+          -- We expect a UP contradiction under the new assignment
           split at h_loop
-          · simp at h_loop
-          · rename_i ri h_ri h_find_hint
-            -- What's the result of assuming the negation of the reduced clause?
-            split at h_loop
-            <;> rename_i τ'' h_assume
-            · -- Error: the clause is satisfied by σ or τ
-              rcases assumeRATClause_error h_models hC h_assume with ⟨hτ_le, hτ_ext⟩
-              clear h_assume
-              have : line.ratHints.size + 1 - bc = line.ratHints.size - (bc + 1) + 2 := by omega
-              rcases uniform_bump_of_uniform_of_extendsFor' (this ▸ h_uniform) hτ_ext with ⟨h_uniform'', hτ''⟩
-              clear this
-              have : (line.ratHints.size - (bc + 1) + 1) = line.ratHints.size + 1 - (bc + 1) := by omega
-              rw [this] at h_uniform''
-              rcases ih hj' h_uniform'' h_loop with ⟨hτ, hpf, hkC⟩
-              clear ih
-              rcases hτ with ⟨b, hb₁, hb₂⟩
-              use ⟨b, by omega, hb₂⟩
-              clear b hb₁ hb₂
-              use Eq.trans hpf hτ''.symm
-              intro k hk₂ C' hC' hk₁
-              rcases lt_or_eq_of_le hk₁ with (hk₁ | rfl)
-              · rw [hτ'']
-                exact hkC hC' (Nat.succ_le_of_lt hk₁)
-              · simp [hC'] at hC
-                subst hC
-                exact inf_le_of_right_le hτ_le
-            · -- .ok: we assumed the negation of the clause under σ
-              -- We expect a UP contradiction under the new assignment
-              split at h_loop
-              <;> try simp at h_loop
-              rename_i τ''' h_up
-              rcases applyUPHints_contra h_models h_up with ⟨h_bot, h_ext₃⟩
-              rcases assumeRATClause_ok h_models hC h_assume with ⟨hτ'', h_ext⟩
-              have : (line.ratHints.size + 1 - bc) = (line.ratHints.size - (bc + 1) + 2) := by omega
-              rcases uniform_bump_of_uniform_of_extendsFor' (this ▸ h_uniform) h_ext with ⟨h_uniform'', hpf⟩
-              clear this
-              have : (line.ratHints.size - (bc + 1) + 1) = line.ratHints.size + 1 - (bc + 1) := by omega
-              rw [this] at h_uniform''
-              clear this
-              have h_ext₄ := extendsFor_trans h_ext h_ext₃
-              have h_uniform''' : τ'''.bump.uniform (line.ratHints.size + 1 - (bc + 1)) := by
-                have h_uni : uniform τ (line.ratHints.size - (bc + 1) + 2) := by
-                  have : (line.ratHints.size + 1 - bc) = (line.ratHints.size - (bc + 1) + 2) := by omega
-                  exact this ▸ h_uniform
-                have h_uni' := (uniform_bump_of_uniform_of_extendsFor' (τ₁ := τ) (τ₂ := τ''')
-                    (offset := line.ratHints.size - (bc + 1)) h_uni h_ext₄).1
-                have : (line.ratHints.size - (bc + 1) + 1) = line.ratHints.size + 1 - (bc + 1) := by omega
-                exact this ▸ h_uni'
-              have hpf₄ : τ.toPropFun = τ'''.bump.toPropFun := by
-                have h_uni : uniform τ (line.ratHints.size - (bc + 1) + 2) := by
-                  have : (line.ratHints.size + 1 - bc) = (line.ratHints.size - (bc + 1) + 2) := by omega
-                  exact this ▸ h_uniform
-                exact (uniform_bump_of_uniform_of_extendsFor' (τ₁ := τ) (τ₂ := τ''')
-                    (offset := line.ratHints.size - (bc + 1)) h_uni h_ext₄).2
-              rcases ih hj' h_uniform''' h_loop with ⟨⟨b, hb₁, hb₂⟩, hpf₃, hkC⟩
-              use ⟨b, by omega, hb₂⟩, Eq.trans hpf₃ hpf₄.symm
-              clear b hb₁ hb₂
-              intro k hk₂ C' hC' hk₁
-              rcases lt_or_eq_of_le hk₁ with (hk₁ | rfl)
-              · simpa [hpf₄] using hkC hC' (Nat.succ_le_of_lt hk₁)
-              · simp [hC'] at hC
-                subst hC
-                apply le_iff_inf_compl_eq_bot.mpr
-                rwa [inf_assoc, ← clauseAsListToPropFun, ← hτ'']
-        · simp at h_loop
+          <;> try simp at h_loop
+          rename_i τ''' h_up
+          rcases applyUPHints_contra h_models h_up with ⟨h_bot, h_ext₃⟩
+          clear h_up
+          have h_bc2 : (line.ratHints.size + 1 - bc) = (line.ratHints.size - (bc + 1) + 2) := by omega
+          have h_ext₄ := extendsFor_trans h_ext h_ext₃
+          rcases uniform_bump_of_uniform_of_extendsFor' (h_bc2 ▸ h_uniform) h_ext with ⟨h_uniform₃, hpf₃⟩
+          clear h_uniform₃
+          rcases uniform_bump_of_uniform_of_extendsFor' (h_bc2 ▸ h_uniform) h_ext₄ with ⟨h_uniform₄, hpf₄⟩
+          have h_bc1 : (line.ratHints.size - (bc + 1) + 1) = line.ratHints.size + 1 - (bc + 1) := by omega
+          rw [h_bc1] at h_uniform₄
+          rw [hpf₄] at hτ'' ⊢
+          rcases ih (Nat.succ_le_of_lt hi_lt) hj' h_uniform₄ h_loop with ⟨⟨b, hb₁, hb₂⟩, hpf₃, hL, hC⟩
+          refine ⟨⟨b, by omega, hb₂⟩, hpf₃, ?_, hC⟩
+          clear ih h_find_hint h_loop hpf₄ b hb₁ hb₂ hpf₃ hC
+          simp [← List.getElem_cons_drop hi_lt', hC, hL]
+          clear hC hL
+          apply le_iff_inf_compl_eq_bot.mpr
+          simp at hτ''
+          rw [inf_assoc, ← hτ'']
+          exact h_bot
+
+theorem checkLine.loop_true {F : RangeArray ILit} {τ τ' : PPA}
+    {Ls : List (Option (List ILit))} {L : List ILit} (h_models : models F Ls L)
+    {σ : PS} {line : SRAdditionLine}
+  : uniform τ (line.ratHints.size + 1) →
+    checkLine.loop F line.witnessMaps line.ratHintIndexes line.ratHints line.ratSizesEq σ 0 (Nat.zero_le _) 0 0 τ
+      = ⟨τ', true⟩ →
+        (cnfAsListToPropFun Ls) ⊓ τ ≤ PropFun.substL (cnfAsListToPropFun Ls) σ.toSubst
+      ∧ (cnfAsListToPropFun Ls) ⊓ τ ≤ PropFun.substL (clauseAsListToPropFun L) σ.toSubst := by
+  intro h_uniform h_loop
+  have : F.size = F.size - 0 := by exact Eq.symm (Nat.sub_zero F.size)
+  conv at h_uniform => rhs; rw [← Nat.sub_zero (line.ratHints.size + 1)]
+  rcases checkLine.loop_true_aux h_models (Nat.zero_le _) this h_uniform h_loop with ⟨hb, hτ', hL, hC⟩
+  clear hb h_loop
+  simp at hL
+  exact ⟨hL, hC⟩
 
 -- The SR rule
 theorem eqsat_of_SR {F C : PropFun ν} :
@@ -924,7 +1061,6 @@ theorem eqsat_of_SR {F C : PropFun ν} :
 theorem eqsatL_of_SR {F C : PropFun ν} :
     (∃ σ, F ⊓ Cᶜ ≤ substL (F ⊓ C) σ) → EquiSat F (F ⊓ C) := by
   rintro ⟨σ, hSR⟩
-  stop
   constructor
   · rintro ⟨τ, hτF⟩
     by_cases hτC : τ ⊨ C
@@ -932,12 +1068,11 @@ theorem eqsatL_of_SR {F C : PropFun ν} :
       rw [satisfies_conj]
       exact ⟨hτF, hτC⟩
     · replace hSR := entails_ext.mp hSR τ
-      simp [satisfies_conj, and_imp, -satisfies_substL] at hSR
-      replace hSR := hSR hτF hτC
-      use PropAssignment.substL (liftSubstL σ) τ
-      rw [satisfies_conj]
-      simp [← subst_liftSubst_eq_substL] at hSR
-      exact hSR
+      have hτFC : τ ⊨ F ⊓ Cᶜ := by
+        simpa [satisfies_conj] using And.intro hτF hτC
+      have hSubst : τ ⊨ substL (F ⊓ C) σ := hSR hτFC
+      use τ.subst (⟦σ ·⟧)
+      simpa [satisfies_substL] using hSubst
   · rintro ⟨τ, hτ⟩
     rw [satisfies_conj] at hτ
     exact ⟨τ, hτ.1⟩
@@ -948,94 +1083,159 @@ theorem checkLine_spec {F : RangeArray ILit}
   : match checkLine ⟨F, τ, σ⟩ line with
     | .error false => True
     | .error true => (cnfAsListToPropFun Ls) = ⊥
-    | .ok ⟨F', τ', σ'⟩ =>
+    | .ok ⟨F', _, _⟩ =>
       F' = F.commit
       ∧ PropFun.EquiSat (cnfAsListToPropFun Ls) (cnfAsListToPropFun Ls ⊓ clauseAsListToPropFun L)
   := by
-  -- structure SRAdditionLine where
-  -- witnessLits : Array ILit     -- Maps literals to true/false
-  -- witnessMaps : Array ILit     -- Maps variables to literals
-  -- upHints : Array Nat          -- Already 0-indexed clause IDs into the accumulated formula
-  -- ratHintIndexes : Array Nat   -- Already 0-indexed
-  -- ratHints : Array (Array Nat) -- Already 0-indexed
-  -- ratSizesEq : ratHintIndexes.size = ratHints.size
-  -- witnessMapsMod : witnessMaps.size % 2 = 0
-  --have ⟨witnessLists, witnessMaps, c, d, e, f, g⟩ := line
   unfold checkLine
   simp [assumeNegatedCandidateFor_eq_assumeNegatedClauseFor _ _ h_models]
-  match hC : τ.reset.assumeNegatedClauseFor { toList := L } (line.ratHints.size + 1) with
-  | .error τ' => simp
-  | .ok τ' =>
+  -- Assume the negation of the candidate clause
+  cases h_assume_negated : τ.reset.assumeNegatedClauseFor { toList := L } (line.ratHints.size + 1)
+  <;> simp
+  rename_i τ₂
+  rcases assumeNegatedClauseFor_ok h_assume_negated with ⟨hτ₂, h_ext₂⟩
+  clear h_assume_negated
+  simp at hτ₂
+  -- Apply global UP hints
+  match h_hints : F.applyUPHints (line.ratHints.size + 1) τ₂ line.upHints with
+  | ⟨τ₃, .err⟩ => simp
+  | ⟨τ₃, .contra⟩ =>
+    -- Contradiction. No SR check needed, was a RUP clause
+    rcases applyUPHints_contra h_models h_hints with ⟨hτ₂_bot, h_ext⟩
+    clear h_hints
+    by_cases h_usize : F.usize = 0
+    <;> simp [h_usize]
+    -- The candidate is empty, meaning the formula is UNSAT.
+    · simp [h_models.h_size₂] at h_usize
+      subst h_usize
+      simp at hτ₂
+      simp [hτ₂] at hτ₂_bot
+      exact hτ₂_bot
+    -- The candidate is nonempty, meaning the candidate is RUP.
+    · apply equisat_of_entails
+      simp [hτ₂] at hτ₂_bot
+      exact le_iff_inf_compl_eq_bot.mpr hτ₂_bot
+  | ⟨τ₃, .unit⟩ =>
+    -- We derived units, but no contradiction. SR checking continues.
+    -- First: the candidate *must* be nonempty.
+    by_cases h_usize : F.usize = 0
+    <;> simp [h_usize]
+    have h_usize' : 0 < F.usize := by omega
+    -- Does the call to `loop` return an error?
+    split
+    <;> try exact True.intro
+    all_goals (
+      rename_i h_state
+      -- Is the first witness literal the pivot?
+      split at h_state
+      <;> try simp at h_state
+    )
+    rename_i τ₄ h_loop
+    rcases h_state with ⟨rfl, rfl, rfl⟩
+    apply And.intro rfl
+    rcases applyUPHints_unit h_models h_hints with ⟨hτ₃, h_ext₃⟩
+    clear h_hints
+    replace h_ext₃ := extendsFor_trans h_ext₂ h_ext₃
+    have h_uniform₃ := uniform_of_extendsFor_reset h_ext₃
+    rcases checkLine.loop_true h_models h_uniform₃ h_loop with ⟨hL₃, hC₃⟩
+    clear h_loop h_uniform₃
+    apply eqsatL_of_SR
+    use (assumeWitness σ line.witnessLits line.witnessMaps).toSubst
+    rw [substL_conj, le_inf_iff, ← hτ₂]
+    have := inf_le_inf (le_refl (cnfAsListToPropFun Ls)) hτ₃
+    rw [← inf_assoc, Std.min_self] at this
+    exact ⟨le_trans this hL₃, le_trans this hC₃⟩
+
+theorem checkLine_ok {F F' : RangeArray ILit}
+    {Ls : List (Option (List ILit))} {L : List ILit} (h_models : models F Ls L)
+    (τ τ' : PPA) (σ σ': PS) (line : Trestle.Parsing.SRAdditionLine)
+  : checkLine ⟨F, τ, σ⟩ line = .ok ⟨F', τ', σ'⟩ →
+    F' = F.commit
+    ∧ PropFun.EquiSat (cnfAsListToPropFun Ls) (cnfAsListToPropFun Ls ⊓ clauseAsListToPropFun L) := by
+  intro h
+  have := checkLine_spec h_models τ σ line
+  simp [h] at this
+  exact this
+
+theorem checkLine_error_true {F : RangeArray ILit}
+    {Ls : List (Option (List ILit))} {L : List ILit} (h_models : models F Ls L)
+    (τ : PPA) (σ : PS) (line : Trestle.Parsing.SRAdditionLine)
+  : checkLine ⟨F, τ, σ⟩ line = .error true →
+    (cnfAsListToPropFun Ls) = ⊥ := by
+  intro h
+  have := checkLine_spec h_models τ σ line
+  simp [h] at this
+  exact this
+
+/-! # consumeDeletionLine correctness -/
+
+theorem consumeDeletionLine.loop.cons_succ' (F : RangeArray ILit) {del : Nat} {dels : List Nat}
+    {i j : Nat}
+  : j = dels.length - i →
+    consumeDeletionLine.loop { toList := del :: dels } (i + 1) F = consumeDeletionLine.loop { toList := dels } i F := by
+  intro hj
+  induction j generalizing F i with
+  | zero =>
+    have h_le := Nat.le_of_sub_eq_zero hj.symm
+    unfold loop
+    simp [not_lt_of_ge h_le]
+  | succ j ih =>
+    have hi : i < dels.length := by
+      apply Nat.lt_of_sub_pos
+      rw [← hj]
+      exact Nat.zero_lt_succ j
+    have hj' : j = dels.length - (i + 1) := by omega
+    unfold consumeDeletionLine.loop
+    simp [hi]
+    -- Is the deletion ID in the formula?
+    split
+    <;> try rfl
+    rename_i h_del_lt
+    -- Has the clause already been deleted?
+    split
+    <;> try rfl
+    rename_i h_not_deleted
+    simp at h_not_deleted
+    exact ih (F.delete dels[i] h_del_lt) hj'
+
+@[simp]
+theorem consumeDeletionLine.loop.cons_succ (F : RangeArray ILit) (del : Nat) (dels : List Nat) (i : Nat)
+  : consumeDeletionLine.loop { toList := del :: dels } (i + 1) F = consumeDeletionLine.loop { toList := dels } i F := by
+  exact @consumeDeletionLine.loop.cons_succ' F del dels i (dels.length - i) (by omega)
+
+-- This is a rather weak theorem.
+-- After all, this spec allows the function to return a formula with all clauses deleted.
+-- A stronger version might specify that deleted clauses are either from `line` or are deleted in the original formula.
+theorem consumeDeletionLine_ok {F F' : RangeArray ILit} {line : SRDeletionLine}
+  {Ls : List (Option (List ILit))} {L : List ILit} (h_models : models F Ls L) :
+    consumeDeletionLine F line = .ok F' →
+      ∃ Ls', models F' Ls' L ∧
+        cnfAsListToPropFun Ls ≤ cnfAsListToPropFun Ls' := by
+  have ⟨clauses⟩ := line
+  unfold consumeDeletionLine
+  induction clauses generalizing F Ls with
+  | nil =>
+    rw [consumeDeletionLine.loop]
     simp
-    have := assumeNegatedClauseFor_spec τ.reset L (line.ratHints.size + 1)
-    simp [hC] at this
-    rcases this with ⟨hτ', hτ_extends⟩
-    match h_hints : F.applyUPHints (line.ratHints.size + 1) τ' line.upHints with
-    | ⟨τ'', .err⟩ => simp
-    | ⟨τ'', .unit⟩ =>
-      -- We derived units, but no contradiction. SR checking continues.
-      simp
-      by_cases h_usize : F.usize = 0
-      <;> simp [h_usize]
-      · have h_usize' : 0 < F.usize := by omega
-        split
-        · rename_i h
-          split at h
-          · rename_i h_pivot
-            split at h
-            · clear h
-              rename_i τ' h_loop
-
-              done
-            done
-          done
-        done
-      split
-      ·
-        done
-      by_cases h_dsize : F.dsize < F.data.size
-      <;> simp [h_dsize]
-      -- Check that we have a nontrivial witness
-      have h_usize : 0 < F.usize := by
-        simp [usize]; exact h_dsize
-      by_cases h_pivot : line.witnessLits[0]?.getD (F.uget 0 h_usize) = F.uget 0 h_usize
-      <;> simp [h_pivot]
-      split <;> try simp
-      rename_i h_loop
-      split at h_loop
-      <;> try (injection h_loop; contradiction)
-      · simp at h_loop
-      rename_i F' τ' σ' h_loop
-      split at h_loop
-      <;> simp at h_loop
-      -- Now check all the RAT/SR hints
-      rcases h_loop with ⟨rfl, rfl, rfl⟩
-      rename_i τ''' h_loop
-      simp
-      apply eqsat_of_SR'
-      use (assumeWitness σ (F.uget 0 h_usize) line.witnessLits line.witnessMaps).toSubst
-
-      done
-    | ⟨τ'', .contra⟩ =>
-      simp
-      have := applyUPHints_spec (τ := τ') h_models (line.ratHints.size + 1) line.upHints.toList
-      simp [h_hints] at this
-      rcases this with ⟨h_hints₁, h_hints₂⟩
-      by_cases h_usize : F.usize = 0
-      -- Trivial branch: If the candidate is empty, we should have found contradiction by now
-      · simp [h_usize]
-        simp [h_models.h_size₂] at h_usize
-        subst h_usize
-        simp at hτ'
-        simp [hτ'] at h_hints₁
-        exact h_hints₁
-      -- UP Contradiction branch: we return immediately; check for equisat
-      · simp [h_usize]
-        apply equisat_of_entails
-        simp [hτ'] at h_hints₁
-        exact le_iff_inf_compl_eq_bot.mpr h_hints₁
-      done
-    done
-  done
+    rintro rfl
+    use Ls
+  | cons clauseId clauses ih =>
+    unfold consumeDeletionLine.loop
+    simp at ih ⊢
+    intro h_loop
+    -- Check that the clause ID to be deleted is in range
+    split at h_loop
+    <;> try simp at h_loop
+    rename_i h_id_lt
+    rw [h_models.h_size₁] at h_id_lt
+    -- Check that the clause ID is not already deleted
+    split at h_loop
+    <;> try simp at h_loop
+    rename_i h_not_deleted
+    simp at h_not_deleted
+    have := models_delete h_models h_id_lt
+    rcases ih this h_loop with ⟨Ls', h_models', hpf⟩
+    use Ls', h_models'
+    exact le_trans (cnfPropFun_le_set_none h_id_lt) hpf
 
 end Trestle.SR
